tests/fir/run.sh
@@ -81,6 +81,8 @@ run_case tests/fir/generic_direct_call.facet "call %t0#0 as affine isize = id#0 
 run_case tests/valid/struct/basic_literal.facet "Pair { x = 1 as unrestricted isize, y = true as unrestricted bool } as unrestricted Pair"
 run_case tests/fir/enum_match.facet "match b#1 as unrestricted BoolLike { Yes => match_Yes_"
 run_case tests/fir/enum_match.facet "No => match_No_"
+run_case tests/fir/enum_structural_no_payload_match.facet "match d#1 as unrestricted Direction { North => match_North_"
+run_case tests/fir/enum_structural_no_payload_match.facet "West => match_West_"
 run_case tests/valid/struct/basic_literal.facet "project %t0#0 as unrestricted isize = p#1.x as unrestricted isize"
 run_case tests/fir/struct_field_borrow.facet "borrow %t0#0 = &p#1.y as unrestricted bool"
 run_case tests/fir/nested_field_access.facet "project %t0#0 as unrestricted isize = o#1.inner.value as unrestricted isize"
